

TP 3: Hastings - Metropolis and Gibbs samplers

①

Kevin
Wardabhan

Exercise 1: 1.A - A population model for longitudinal data

1)

We consider $\Theta = (\bar{\mu}_0, \bar{\sigma}_0, \sigma_\varepsilon, \sigma_\tau, \sigma)$ and $z := ((z_i)_{i \in \{1, \dots, N\}}, \mathbf{z}_{pp})$
where $N \in \mathbb{N}^*$.
 $\in \mathbb{R}^{2N+2}$

The complete data log-likelihood is:

$$\log(q(y, z, \theta)) = \underbrace{\log(q(y|z, \theta))}_{(1)} + \underbrace{\log(q(z|\theta))}_{(2)} + \underbrace{\log(q(\theta))}_{(3)}$$

Let's compute each term separately.

$$\begin{aligned} (3) = \log(q(\theta)) &= \log(q(\bar{\mu}_0, \bar{\sigma}_0, \sigma_\varepsilon, \sigma_\tau, \sigma)) \\ \text{(priors are supposed independent)} \quad (3) &= \log(q(\bar{\mu}_0)) + \log(q(\bar{\sigma}_0)) + \sum_{\tilde{\sigma} \in \{\sigma_\varepsilon, \sigma_\tau, \sigma\}} \log(q(\tilde{\sigma})) \\ &= -\frac{1}{2\delta_{\mu_0}^2} (\bar{\mu}_0 - \bar{\mu}_0)^2 - \frac{1}{2\delta_{\sigma_0}^2} (\bar{\sigma}_0 - \bar{\sigma}_0)^2 + \sum_{\tilde{\sigma} \in \{\sigma_\varepsilon, \sigma_\tau, \sigma\}} \log(q(\tilde{\sigma})) + C_1 \end{aligned}$$

$$\text{where } C_1 = -\frac{1}{2} [\log(2\pi\delta_{\mu_0}^2) + \log(2\pi\delta_{\sigma_0}^2)] \in \mathbb{R}$$

Moreover,

$$\sum_{\tilde{\sigma} \in \{\sigma, \sigma_g, \sigma_\tau\}} \log(q(\tilde{\sigma})) = -\log(\sigma^2) - \log(\sigma_\tau^2) - \log(\sigma_g^2)$$

$$+ m_g \log\left(\frac{v_g}{\sigma_g}\right) + m_\tau \log\left(\frac{v_\tau}{\sigma_\tau}\right) + m \log\left(\frac{v}{\sigma}\right) - \frac{v_g^2}{2\sigma_g^2} - \frac{v_\tau^2}{2\sigma_\tau^2} - \frac{v^2}{2\sigma^2} + c_2$$

where $c_2 = -\log\left(\Gamma\left(\frac{m_g}{2}\right)\right) - \log\left(\Gamma\left(\frac{m_\tau}{2}\right)\right) - \log\left(\Gamma\left(\frac{m}{2}\right)\right)$

$$+ m_g \log\left(\frac{1}{\sqrt{2}}\right) + m_\tau \log\left(\frac{1}{\sqrt{2}}\right) + m \log\left(\frac{1}{\sqrt{2}}\right)$$

Thus, $\log(q(\theta)) = -\frac{1}{2\sigma_{\tau_0}^2} (\bar{t}_0 - \bar{t}_0)^2 - \frac{1}{2\sigma_{\tau_0}^2} (\bar{v}_0 - \bar{v}_0)^2$

$$+ m_g \log\left(\frac{v_g}{\sigma_g}\right) - \log(\sigma_g^2) - \frac{v_g^2}{2\sigma_g^2}$$

$$+ m_\tau \log\left(\frac{v_\tau}{\sigma_\tau}\right) - \log(\sigma_\tau^2) - \frac{v_\tau^2}{2\sigma_\tau^2}$$

$$+ m \log\left(\frac{v}{\sigma}\right) - \log(\sigma^2) - \frac{v^2}{2\sigma^2} + c_3$$

where $c_3 = c_1 + c_2$.

Exercise 1:

(2)

1) We now compute (2).

$$(2) = \log(q(z|\theta)) = \left[\sum_{i=1}^N \log(q(z_i|\theta)) \right] + \log(q(z_{\text{pop}}|\theta))$$

First, $\log(q(z_{\text{pop}}|\theta)) = \log(q(t_0, v_0 | \bar{t}_0, \bar{v}_0))$

$$\left(\begin{array}{l} t_0 \sim \mathcal{N}(\bar{t}_0, \sigma_{t_0}^2) \\ v_0 \sim \mathcal{N}(\bar{v}_0, \sigma_{v_0}^2) \\ t_0 \perp v_0 \end{array} \right) \quad \hookrightarrow \quad = \log(q(t_0 | \bar{t}_0)) + \log(q(v_0 | \bar{v}_0))$$

$$= -\frac{1}{2\sigma_{t_0}^2} (t_0 - \bar{t}_0)^2 - \frac{1}{2\sigma_{v_0}^2} (v_0 - \bar{v}_0)^2 + C_4$$

where $C_4 = -\frac{1}{2} [\log(2\pi\sigma_{t_0}^2) + \log(2\pi\sigma_{v_0}^2)] \in \mathbb{R}$

Plus, $\forall i \in [1, N]$,
 $(t_i, d_i \perp \tau_i)$

$$\log(q(z_i|\theta)) \stackrel{\hookrightarrow}{=} \log(q(d_i|\theta)) + \log(q(\tau_i|\theta))$$

$$\begin{array}{l} d_i \sim \text{LogN}(0, \sigma_d^2) \\ \tau_i \stackrel{\text{iid}}{\sim} \mathcal{N}(0, \sigma_\tau^2) \end{array} \quad = -\log(d_i) - \frac{\log(d_i)^2}{2\sigma_d^2} - \frac{1}{2\sigma_\tau^2} \tau_i^2 - \log(\sigma_d \sigma_\tau) + C_5$$

where $C_5 = -\log(2\pi)$

Thus,

$$q(z|\theta) = - \left[\sum_{i=1}^N \log(d_i) + \frac{\log(d_i)^2}{2\sigma_g^2} + \frac{\tau_i^2}{2\sigma_\tau^2} \right] - N \log(\sigma_g \sigma_\tau) \\ - \frac{1}{2\sigma_{t_0}^2} (t_0 - \bar{t}_0)^2 - \frac{1}{2\sigma_{v_0}^2} (v_0 - \bar{v}_0)^2 + C_6$$

where $C_6 = C_4 + NC_5$.

Finally, we compute (I)

$$(I) = \log(q(y|z, \theta)) = \sum_{i=1}^N \log(q(y_i|z, \theta)) \\ = \sum_{i=1}^N \sum_{j=1}^{b_i} \log(q(y_{ij}|z, \theta))$$

$\forall i \in [1, N], \forall j \in [1, b_i], y_{ij} \sim \mathcal{N}(d_i(t_{ij}), \sigma^2)$, so

$$\log(q(y_{ij}|z, \theta)) = -\frac{1}{2\sigma^2} (y_{ij} - d_i(t_{ij}))^2 - \frac{1}{2} \log(\sigma^2) + C_7$$

where $C_7 = -\frac{1}{2} \log(2\pi)$

$$\text{So, } \log(q(y|z, \theta)) = \sum_{i=1}^N \sum_{j=1}^{b_i} \left[-\frac{1}{2\sigma^2} (y_{ij} - d_i(t_{ij}))^2 - \frac{1}{2} \log(\sigma^2) \right] + C_8$$

where $C_8 = \sum_{i=1}^N \sum_{j=1}^{b_i} C_7 = C_7 \sum_{i=1}^N b_i$

Exercise 1:

(3)

1) Finally, we obtain that:

$$\log(q(y, z; \theta)) = \sum_{i=1}^N \sum_{j=1}^{b_i} \left[-\frac{1}{2\sigma^2} (y_{ij} - d_i | t_{ij})^2 - \frac{1}{2} \log(\sigma^2) \right]$$

$$+ \sum_{i=1}^N \left[-\log(d_i) - \frac{\log(d_i)^2}{2\sigma_\xi^2} - \frac{\tau_i^2}{2\sigma_\tau^2} \right] - N \log(\sigma_\xi \sigma_\tau)$$

$$- \frac{1}{2\sigma_{t_0}^2} (t_0 - \bar{t}_0)^2 - \frac{1}{2\sigma_{v_0}^2} (v_0 - \bar{v}_0)^2$$

$$- \frac{1}{2\sigma_{t_0}^2} (\bar{t}_0 - \bar{\bar{t}}_0)^2 - \frac{1}{2\sigma_{v_0}^2} (\bar{v}_0 - \bar{\bar{v}}_0)^2$$

$$+ m_\xi \log\left(\frac{v_\xi}{\sigma_\xi}\right) - \log(\sigma_\xi^2) - \frac{v_\xi^2}{2\sigma_\xi^2}$$

$$+ m_\tau \log\left(\frac{v_\tau}{\sigma_\tau}\right) - \log(\sigma_\tau^2) - \frac{v_\tau^2}{2\sigma_\tau^2}$$

$$+ m \log\left(\frac{v}{\sigma}\right) - \log(\sigma^2) - \frac{v^2}{2\sigma^2} + C$$

where $C = C_1 + C_2 + C_3$

We can write the log-likelihood as

$-\phi(\theta) + S(y, z)^T \psi(\theta) + \log(h(y, z))$ by setting:

$$S(y, z) = \begin{pmatrix} \frac{1}{N_b} \sum_{i=1}^N \sum_{j=1}^{b_i} (y_{ij} - d_i(t_{ij}))^2 \\ \frac{1}{N} \sum_{i=1}^N \log(d_i)^2 \\ \frac{1}{N} \sum_{i=1}^N \tau_i^2 \\ t_0 \\ v_0 \end{pmatrix} \quad (\text{here } N_b = \sum_{i=1}^N b_i)$$

$$\psi(\theta) = \begin{pmatrix} -\frac{N_b}{2\sigma^2} \\ -\frac{N}{2\sigma_g^2} \\ -\frac{N}{2\sigma_\tau^2} \\ \frac{t_0}{\sigma_{t_0}^2} \\ \frac{v_0}{\sigma_{v_0}^2} \end{pmatrix}$$

$$\begin{aligned} \phi(\theta) = & \frac{\bar{t}_0^2}{2\sigma_{t_0}^2} + \frac{\bar{v}_0^2}{2\sigma_{v_0}^2} + \frac{\bar{t}_0^2}{2\sigma_{t_0}^2} + \frac{\bar{v}_0^2}{2\sigma_{v_0}^2} - \frac{\bar{t}_0 \bar{t}_0}{\sigma_{t_0}^2} - \frac{\bar{v}_0 \bar{v}_0}{\sigma_{v_0}^2} \\ & - \frac{N_g^2}{2\sigma_g^2} - \frac{v_\tau^2}{2\sigma_\tau^2} - \frac{v^2}{2\sigma^2} + (N_b + m + 2) \log(\sigma) + (N_b + m_g + 2) \log(\sigma_g) \\ & + (N_b + m_\tau + 2) \log(\sigma_\tau) \end{aligned}$$

Exercise 1.

4) We want to compute for $b \in N$ fixed:

$$\theta^{(b)} = \underset{\theta \in \Theta}{\operatorname{argmax}} \quad \mathcal{V}_b(\theta) := -\phi(\theta) + S_b(y, z)^T \psi(\theta)$$

where $S_b(y, z) = (S_b^{(i)}(y, z))_{i \in \{1, \dots, 5\}}$.

Differentiating $\theta \mapsto \mathcal{V}_b(\theta)$ gives:

$$\nabla \mathcal{V}_b(\theta) = -\nabla \phi(\theta) + J_\psi(\theta)^T S_b(y, z)$$

Moreover:

$$-\nabla \phi(\theta) =$$

$$\begin{pmatrix} \frac{\bar{t}_0}{s_{t_0}^2} - \bar{t}_0 \left(\frac{1}{s_{t_0}^2} + \frac{1}{\sigma_{t_0}^2} \right) \\ \frac{\bar{v}_0}{s_{v_0}^2} - \bar{v}_0 \left(\frac{1}{s_{v_0}^2} + \frac{1}{\sigma_{v_0}^2} \right) \\ \frac{\bar{v}_g^2}{\sigma_g^3} - \frac{(N_b + m_g + 2)}{\sigma_g} \\ \frac{\bar{v}_\tau^2}{\sigma_\tau^3} - \frac{(N_b + m_\tau + 2)}{\sigma_\tau} \\ \frac{\bar{v}^2}{\sigma^3} - \frac{(N_b + m + 2)}{\sigma} \end{pmatrix}$$

and $J_{\psi}(\theta)^T =$

$$\begin{pmatrix} 0 & 0 & 0 & \sigma_{t_0}^{-2} & 0 \\ 0 & 0 & 0 & 0 & \sigma_{v_0}^{-2} \\ 0 & \frac{2}{\sigma_{\epsilon_3}^2} & 0 & 0 & 0 \\ 0 & 0 & \frac{2}{\sigma_{\epsilon_3}^2} & 0 & 0 \\ \frac{N_B}{\sigma^3} & 0 & 0 & 0 & 0 \end{pmatrix}$$

Thus, $\nabla \psi_b(\theta) = 0$

$\Rightarrow \theta_b :=$

$$\begin{pmatrix} t_0 \\ v_0 \\ \sigma_{\epsilon} \\ \sigma_{\tau} \\ \rho \end{pmatrix} = \begin{pmatrix} \left(\frac{\bar{t}_0}{\sigma_{t_0}^2} + \frac{S_b^{(4)}}{\sigma_{t_0}^2} \right) \frac{\sigma_{t_0}^2 \sigma_{t_0}^2}{\sigma_{t_0}^2 + \sigma_{t_0}^2} \\ \left(\frac{\bar{v}_0}{\sigma_{v_0}^2} + \frac{S_b^{(5)}}{\sigma_{v_0}^2} \right) \frac{\sigma_{v_0}^2 \sigma_{v_0}^2}{\sigma_{v_0}^2 + \sigma_{v_0}^2} \\ \frac{S_b^{(2)} N + \sigma_{\epsilon}^2}{N_b + m_{\epsilon} + 2} \\ \frac{S_b^{(3)} N + \sigma_{\tau}^2}{N_b + m_{\tau} + 2} \\ \frac{S_b^{(1)} N + \sigma^2}{N_b + m + 2} \end{pmatrix}$$

Exercise 3: Multiplicative Hastings-Metropolis ①

Let f be a density function on $[-1, 1]$,
a random variable ε having f for distribution
and independent of $B \sim \text{Ber}(\frac{1}{2})$. Let X be
a random variable such that we have mutual
independence of (X, B, ε) .

1) Let's compute the density of the jumping
distribution $Y \sim q(X, Y)$.

Let $\varphi: \mathbb{R} \rightarrow \mathbb{R}$ a Borel bounded function.

$$\mathbb{E}[\varphi(Y) | X] = \mathbb{E}[\varphi(Y) (\mathbb{1}_{\{B=1\}} + \mathbb{1}_{\{B=0\}}) | X]$$

$$= \mathbb{E}[\varphi(Y) \mathbb{1}_{\{B=1\}} | X] + \mathbb{E}[\varphi(Y) \mathbb{1}_{\{B=0\}} | X]$$

$$= g(X) + h(X)$$

$$\text{where } \begin{cases} g(x) = \mathbb{E}[\varphi(Y) \mathbb{1}_{\{B=1\}} | X=x] & \text{i)} \end{cases}$$

$$\begin{cases} h(x) = \mathbb{E}[\varphi(Y) \mathbb{1}_{\{B=0\}} | X=x] & \text{ii)} \end{cases}$$

i) Moreover, $\forall x \neq 0$ (if $x=0$, then $\gamma=0$ a.s)

$$\begin{aligned}
 g(x) &= \mathbb{E}[\varphi(Y) \mathbb{1}_{\{B=1\}} | X=x] \\
 &\quad \downarrow B=1 \text{ a.s.} \\
 &= \mathbb{E}[\varphi(\varepsilon X) \mathbb{1}_{\{B=1\}} | X=x] \\
 &\quad \downarrow (\varepsilon, B) \perp\!\!\!\perp X \\
 &= \mathbb{E}[\varphi(\varepsilon x) \mathbb{1}_{\{B=1\}}] \\
 &\quad \downarrow \varepsilon \perp\!\!\!\perp B \\
 &= \frac{1}{2} \mathbb{E}[\varphi(\varepsilon x)]
 \end{aligned}$$

$$= \frac{1}{2} \int_{-1}^1 \varphi(zx) f(z) dz = \frac{1}{2} \int_{-|x|}^{|x|} \varphi(y) f\left(\frac{y}{x}\right) \frac{1}{|x|} dy$$

by doing the change of variable $\psi:]-1, 1[\rightarrow]-|x|, |x|[$

ii) By doing the same for h , $\left\{ \begin{array}{l} \psi:]-1, 1[\rightarrow]-|x|, |x|[\\ z \mapsto zx =: y \end{array} \right.$
we get: $\forall x \neq 0$,

$$h(x) = \frac{1}{2} \mathbb{E}\left[\varphi\left(\frac{x}{\varepsilon}\right)\right] = \frac{1}{2} \int_{\mathbb{R}} \varphi(y) f\left(\frac{x}{y}\right) \frac{|x|}{y^2} \mathbb{1}_{|x| < |y| < 1} dy$$

by letting the change of variable:

$$\begin{aligned}
 \psi':]-1, 1[&\rightarrow \{y \in \mathbb{R} \mid |x| < |y| < 1\} \\
 z &\mapsto \frac{x}{z} =: y
 \end{aligned}$$

Exercise 3:

(2)

Finally, we get:

$$\mathbb{E}[\ell(Y)|X] = g(x) + h(x)$$

$$= \int_{\mathbb{R}} \ell(y) \left[\frac{1}{2} f\left(\frac{y}{x}\right) \frac{1}{|x|} \mathbb{1}_{|y| < |x|} + f\left(\frac{x}{y}\right) \frac{|x|}{y^2} \mathbb{1}_{|x| < |y| < 1} \right] dy$$

So, $\forall x \neq 0, \forall y \in \mathbb{R}$,

$$q(x, y) = \frac{1}{2} \left[f\left(\frac{y}{x}\right) \frac{1}{|x|} \mathbb{1}_{|y| < |x|} + f\left(\frac{x}{y}\right) \frac{|x|}{y^2} \mathbb{1}_{|x| < |y| < 1} \right]$$

Remark:

If $y=0$, we set the convention $f\left(\frac{x}{y}\right) \frac{|x|}{y^2} \mathbb{1}_{|x| < |y| < 1} = 0$
 $x \neq 0$

so that $q(x, 0) = \frac{1}{2} f(0) \frac{1}{|x|}$

2) We know that the classical Hastings-Metropolis algorithm is:

$$\alpha(x, y) = \begin{cases} \min\left(1, \frac{\pi(y) q(x, y)}{\pi(x) q(y, x)}\right) & \text{if } \pi(x) q(x, y) > 0 \\ 1 & \text{otherwise} \end{cases}$$

where π is a fixed invariant probability measure for the chain.

Let x, y s.t. $q(x, y) > 0$, then:

$$\frac{q(y, x)}{q(x, y)} = \frac{\frac{1}{|y|} f(\frac{x}{y})}{\frac{|x|}{|y|^2} f(\frac{x}{y})} \mathbb{1}_{|x| < |y| < 1} + \frac{\frac{|y|}{x^2} f(\frac{y}{x})}{\frac{1}{|x|} f(\frac{y}{x})} \mathbb{1}_{|y| < |x| < 1}$$

$$= |\frac{y}{x}| \mathbb{1}_{|x| < 1} \mathbb{1}_{|y| < 1} = |\frac{y}{x}|$$

because the chain lives in $\mathbb{J} - 1, 1[$.

So, for a fixed π ,

$$d(x, y) = \begin{cases} \min(1, \frac{\pi(y)}{\pi(x)} |\frac{y}{x}|) & \text{if } x \neq 0 \text{ and } \pi(x) > 0 \\ 1 & \text{otherwise} \end{cases}$$
